\documentclass{article}
\usepackage[fleqn]{amsmath}
\usepackage{tikz}
\tikzset{%
  point/.style={circle,inner sep=1.25pt,minimum size=1.25pt,draw,fill=#1},
  point/.default=red
}
\definecolor{c0}{rgb}{0.2,0.4,0.67}
\definecolor{c1}{rgb}{0.67,0.4,0.12}
\definecolor{c2}{rgb}{0.53,0.6,0.13}
\definecolor{c3}{rgb}{0.53,0.53,0.4}
\begin{document}
\section{General Case}
\begin{align*}
  a_1 x_1 + b_1 y_1 + c_1 & = 0\\
  a_1 x_2 + b_1 y_2 + c_1 & = 0\\
  (x - x_1)^2 + (y - y_1)^2 & = d_1^2\\
  (x - x_2)^2 + (y - y_2)^2 & = d_2^2\\
  (x_2 - x_1)^2 + (y_2 - y_1)^2 & = d_1^2 + d_2^2 - 2 c d_1 d_2 = d_1^2 + d_2^2 - 2 k
\end{align*}
\section{Without Translation ($c_1 = c_2 = 0$)}
\begin{align*}
  y_1 & = m_1 x_1\\
  y_2 & = m_2 x_2\\
  (x - x_1)^2 + (y - m_1 x_1)^2 & = d_1^2\\
  (x - x_2)^2 + (y - m_2 x_2)^2 & = d_2^2\\
  (x_2 - x_1)^2 + (m_2 x_2 - m_1 x_1)^2 & = d_1^2 + d_2^2 - 2 k
\end{align*}
\begin{align*}
  x^2 + x_1^2 - 2 x x_1 + y^2 + m_1^2x_1^2 - 2 y m_1 x_1 &= d_1^2\\
  (1 + m_1^2) x_1^2 - 2 (x + y m_1) x_1  + x^2 + y^2  &= d_1^2\\
  (1 + m_2^2) x_2^2 - 2 (x + y m_2) x_2  + x^2 + y^2  &= d_2^2\\
  x_2^2 + x_1^2 - 2 x_1 x_2 + m_1^2 x_1^2 + m_2^2 x_2^2 - 2 m_1 m_2 x_1 x_2 &= d_1^2 + d_2^2 - 2 k\\
  (1 + m_1^2) x_1^2 + (1 + m_2^2) x_2^2 - 2 (1 - m_1 m_2) x_1 x_2 &= d_1^2 + d_2^2 - 2 k\\
\end{align*}
\begin{align*}
  2 (1 - m_1 m_2) x_1 x_2 - 2 (x + y m_1) x_1 - 2 (x + y m_2) x_2 + 2 x^2 + 2 y^2 &= 2 k
\end{align*}
\section{Orthogonal ($m_1 m_2 = -1$)}
\begin{align*}
  2 x^2 + 2 y^2 - 2 (x + y m_1) x_1 - 2 (x + y m_2) x_2 &= 2 k\\
  (1 + m_1^2) x_1^2 - 2 (x + y m_1) x_1  + x^2 + y^2 - d_1^2 &= 0\\
  (1 + m_2^2) x_2^2 - 2 (x + y m_2) x_2  + x^2 + y^2 - d_2^2 &= 0\\
\end{align*}
\begin{align*}
  x_1 &= \frac{x + y m_1 + \sqrt{(x + y m_1)^2 - (1 + m_1^2)(x^2 + y^2 - d_1^2)}}{(1 + m_1^2)}\\
  x_2 &= \frac{x + y m_2 + \sqrt{(x + y m_2)^2 - (1 + m_2^2)(x^2 + y^2 - d_2^2)}}{(1 + m_2^2)}
\end{align*}
\section{Axis Aligned}
\begin{align*}
  y_1 & = 0\\
  x_2 & = 0\\
  (x - x_1)^2 + y^2 &= d_1^2\\
  x^2 + (y - y_2)^2 &= d_2^2\\
  x_1^2 + y_2^2 &= d_1^2 + d_2^2 - 2 c d_1 d_2 = d_1^2 + d_2^2 - 2 k
\end{align*}
\begin{align*}
  x_1^2 - 2 x x_1 + x^2 + y^2 - d_1^2 &= 0\\
  y_2^2 - 2 y y_2 + x^2 + y^2 - d_2^2 &= 0\\
\end{align*}
\begin{align*}
  x_1 &= x + \sqrt{d_1^2 - y^2)}\\
  y_2 &= y + \sqrt{d_2^2 - x^2)}
\end{align*}
\begin{align*}
  x_1^2 + y_2^2 &= d_1^2 + d_2^2 - 2 k\\
  (x \pm \sqrt{d_1^2 - y^2)})^2 + (y \pm \sqrt{d_2^2 - x^2)})^2 &= d_1^2 + d_2^2 - 2 k\\
  x^2 + d_1^2 - y^2 + y^2 + d_2^2 - x^2 \pm 2 x \sqrt{d_1^2 - y^2)} \pm 2 y \sqrt{d_2^2 - x^2)} &= d_1^2 + d_2^2 - 2 k\\
  \pm x \sqrt{d_1^2 - y^2)} \pm y \sqrt{d_2^2 - x^2)} &= -k\\
  x^2 (d_1^2 - y^2) + y^2 (d_2^2 - x^2) \pm 2 x y \sqrt{d_1^2 - y^2)} \sqrt{d_2^2 - x^2)} &= k^2
\end{align*}
\begin{align*}
  \pm 2 x y \sqrt{(d_1^2 - y^2)(d_2^2 - x^2)} &= k^2 - x^2 (d_1^2 - y^2) - y^2 (d_2^2 - x^2)\\
  4 x^2 y^2 (d_1^2 - y^2)(d_2^2 - x^2) &= (k^2 - d_1^2x^2 + x^2y^2 - d_2^2y^2 + x^2y^2)^2\\
  4 x^2 y^2 (d_1^2d_2^2 - d_1^2x^2 - d_2^2y^2 + x^2y^2) &= (k^2 - d_1^2 x^2 - d_2^2 y^2 + 2 x^2 y^2)^2\\
  4 d_1^2d_2^2 x^2 y^2 - 4 d_1^2 x^4 y^2 - 4 d_2^2 x^2 y^4 + 4 x^4 y^4  &= k^4 + d_1^4 x^4 + d_2^4 y^4 2 + 4 x^4 y^4 \\
                                                                    &- 2 d_1^2 k^2 x^2 - 2 d_2^2 k^2 y^2 + 4 k^2 x^2 y^2 \\
                                                                    &+ 2 d_1^2 d_2^2 x^2 y^2 - 4 d_1^2 x^4 y^2 - 4 d_2^2 x^2 y^4 \\
  %
  d_1^4 x^4 + d_2^4 y^4 - 2 d_1^2 k^2 x^2 - 2 d_2^2 k^2 y^2 + 4 k^2 x^2 y^2 - 2 d_1^2d_2^2 x^2 y^2 + k^4 &= 0
\end{align*}
\begin{align*}
  (A_1 x^2 + B_1 y^2 + C_1 x y + D_1)(A_2 x^2 + B_2 y^2 + C_2 x y + D_2) &= 0\\
  A_1 A_2 X^4 + B_1 B_2 y^4 + (A_1 C_2 + A_2 C_1) x^3 y + (B_1 C_2 + B_2 C_1) x y^3 + \\
  (A_1 B_2 + A_2 B_1 + c_1 C_2) x^2 y^2 + (A_1 D_2 + A_2 D_1) x^2 + (B_1 D_2 + B_2 D_1) y^2 + \\
  (C_2 D_1 + C_1 D_2) x y + D_1 D_2 &= 0
\end{align*}
\begin{align*}
  A_1 A_2 &= d_1^4\\
  B_1 B_2 &= d_2^4\\
  A_1 C_2 + A_2 C_1 &= 0\\
  B_1 C_2 + B_2 C_1 &= 0\\
  A_1 B_2 + A_2 B_1 + C_1 C_2 &= 4 k^2 - 2 d_1^2 d_2^2\\
  A_1 D_2 + A_2 D_1 &= 2 -d_1^2 k^2\\
  B_1 D_2 + B_2 D_1 &= 2 -d_2^2 k^2\\
  C_2 D_1 + C_1 D_2 &= 0\\
  D_1 D_2 &= k^4
\end{align*}
\begin{align*}
  A_1 &= A_2 = d_1^2\\
  B_1 &= B_2 = d_2^2\\
  C_1 &= -C_2 = 2 \sqrt{d_1^2 d_2^2 - k^2}\\
  D_1 &= D_2 = -k^2\\
\end{align*}
\end{document}
