% =============================================================================
\section{Derivation}
\label{sec:derivation}
% =============================================================================
We repeat the system equation in the general case:
\begin{align}
  a_1 x_1 + b_1 y_1 + c_1 &= 0\\
  a_1 x_2 + b_1 y_2 + c_1 &= 0\\
  (x - x_1)^2 + (y - y_1)^2 &= d_1^2\label{eq:1}\\
  (x - x_2)^2 + (y - y_2)^2 &= d_2^2\label{eq:2}\\
  (x_2 - x_1)^2 + (y_2 - y_1)^2 &= d_1^2 + d_2^2 - 2 c d_1 d_2 = d_1^2 + d_2^2 - 2 k\label{eq:3}
\end{align}

% -----------------------------------------------------------------------------
\subsection{Constraining the Intersection Point}
\label{ssec:derivation-constraining-origin}
% -----------------------------------------------------------------------------
\setlength{\parskip}{1ex}
%\noindent
We set $c_1 = c_2 = 0$, coercing the intersection point of $L_1$ and $L_2$ to coincide with the origin, and denote $m_1 = \frac{a_1}{b_1}$ and $m_2 = \frac{a_2}{b_2}$; we get $y_1 = m_1 x_1$ and $y_2 = m_2 x_2$.

\noindent
We substitute $y_1$ and $y_2$ in equations~\ref{eq:1}, \ref{eq:2}, and \ref{eq:3} and get:
\begin{align}
  (x - x_1)^2 + (y - m_1 x_1)^2 & = d_1^2\\
  (x - x_2)^2 + (y - m_2 x_2)^2 & = d_2^2\\
  (x_2 - x_1)^2 + (m_2 x_2 - m_1 x_1)^2 & = d_1^2 + d_2^2 - 2 k
\end{align}

\noindent
We expand and regroup and get:
\begin{align}
  %x^2 + x_1^2 - 2 x x_1 + y^2 + m_1^2x_1^2 - 2 m_1 y x_1 &= d_1^2\\
  (1 + m_1^2) x_1^2 - 2 (x + m_1 y) x_1  + x^2 + y^2  &= d_1^2\label{eq:d1}\\
  (1 + m_2^2) x_2^2 - 2 (x + m_2 y) x_2  + x^2 + y^2  &= d_2^2\label{eq:d2}\\
  % x_2^2 + x_1^2 - 2 x_1 x_2 + m_1^2 x_1^2 + m_2^2 x_2^2 - 2 m_1 m_2 x_1 x_2 &= d_1^2 + d_2^2 - 2 k\\
  (1 + m_1^2) x_1^2 + (1 + m_2^2) x_2^2 - 2 (1 + m_1 m_2) x_1 x_2 &= d_1^2 + d_2^2 - 2 k\label{eq:d}
\end{align}

\noindent
We substitute $d_1$ and $d_2$ in Equation~\ref{eq:d} and obtain the single equation:
\begin{align}
  % 2 (1 + m_1 m_2) x_1 x_2 - 2 (x + m_1 y) x_1 - 2 (x + m_2 y) x_2 + 2 x^2 + 2 y^2 &= 2 k\\
  (1 + m_1 m_2) x_1 x_2 - (x + m_1 y) x_1 - (x + m_2 y) x_2 + x^2 + y^2 - k &= 0\label{eqs}
\end{align}

% -----------------------------------------------------------------------------
\subsection{Constraining the Slope of One Line}
\label{ssec:derivation-constraining-slope}
% -----------------------------------------------------------------------------
We set $m_1 = 0$ in equations~\ref{eq:d1}, \ref{eq:d2}, and \ref{eqs}, coercing $L_1$ to lie on the $x$-axis, andd get:
\begin{align}
  (x - x_1)^2 + y^2 & = d_1^2\label{eq:d1-s}\\
  (x - x_2)^2 + (y - m_2 x_2)^2 & = d_2^2\label{eq:d2-s}\\
  x_1 x_2 - x x_1 - (x + m_2 y) x_2 + x^2 + y^2 - k &= 0\label{eq:d-s}
\end{align}

\noindent
We solve the quadratic equations~\ref{eq:d1-s} and~\ref{eq:d2-s}, and get:
\begin{align*}
  x_1 &= x \pm \sqrt{d_1^2 - y^2}\\
  x_2 &= \frac{x + m_2 y \pm \sqrt{(x + m_2 y)^2 - (1 + m_2^2)(x^2 + y^2 - d_2^2)}}{1 + m_2^2}\\
  &= \frac{x + m_2 y \pm \sqrt{(2 m_2 x y - y^2 + d_2^2 - m_2^2 x^2 + d_2^2 m_2^2}}{1 + m_2^2}\\
  &= \frac{x + m_2 y}{1 + m_2^2} + \sqrt{\frac{2 m_2 x y - y^2 + d_2^2 - m_2^2 x^2 + d_2^2 m_2^2}{(1 + m_2^2)^2}}
\end{align*}

\noindent
We introduce the symbols $r_1$, $s_1$, $r_2$, and $s_2$, and set
\begin{align*}
  x_1 &= r_1 \pm \sqrt{s_1} = x \pm \sqrt{d_1^2 - y^2}\\
  x_2 &= r_2 \pm \sqrt{s_2}
\end{align*}

\noindent
We substitute $x_1$ and $x_2$ in Equation~\ref{eq:d-s} and get:
\begin{align*}
  % x_1 x_2 - x x_1 - (x + m_2 y) x_2 + x^2 + y^2 - k &= 0\\
  (x \pm \sqrt{s_1}) (r_2 \pm \sqrt{s_2}) - x (x \pm \sqrt{s_1}) - (x + m_2 y) (r_2 \pm \sqrt{s_2}) + x^2 + y^2 - k &= 0\\
\end{align*}

\noindent
We expand and get:
\begin{align*}
  x r_2 \pm x \sqrt{s_2} \pm r_2 \sqrt{s_1} + \sqrt{s_1 s_2} - x^2 \mp x\sqrt{s_1} - r_2 (x + m_2 y) \mp (x + m_2 y)\sqrt{s_2} + x^2 + y^2 - k &= \\
  x r_2 \pm x \sqrt{s_2} \pm r_2 \sqrt{s_1} + \sqrt{s_1 s_2} \mp x\sqrt{s_1} - r_2 x - r_2 m_2 y \mp x \sqrt{s_2} \mp m_2 y\sqrt{s_2}  + y^2 - k &= \\
  \pm r_2 \sqrt{s_1} + \sqrt{s_1 s_2} \mp x\sqrt{s_1} - r_2 m_2 y \mp m_2 y\sqrt{s_2}  + y^2 - k &= 0\\
\end{align*}

\noindent
We remove vanishig terms and regroup and get:
\begin{align*}
  \mp x\sqrt{s_1} \pm r_2 \sqrt{s_1} \mp m_2 y \sqrt{s_2} + \sqrt{s_1 s_2} - r_2 m_2 y + y^2 - k &= 0\\
  \mp (x - r_2) \sqrt{s_1} \mp m_2 y \sqrt{s_2} + \sqrt{s_1 s_2} - r_2 m_2 y + y^2 - k &= 0\\
\end{align*}

\noindent
We exchange and get:
\begin{align*}
  \sqrt{s_1 s_2} + (y^2 - r_2 m_2 y - k) &= \pm (x - r_2) \sqrt{s_1} \pm m_2 y \sqrt{s_2}\\
\end{align*}

\noindent
We raise to the power of two each side and get:
\begin{align*}
  s_1 s_2 + (y^2 - r_2 m_2 y - k)^2 + 2 (y^2 - r_2 m_2 y - k) \sqrt{s_1 s_2}
  &= (x - r_2)^2 s_1 + m_2^2 y^2 s_2 + 2 m_2 y (x - r_2) \sqrt{s_1 s_2}\\
  &= (x - r_2)^2 s_1 + m_2^2 y^2 s_2 + 2 (m_2 x y - r_2 m_2 y) \sqrt{s_1 s_2}\\
\end{align*}

\noindent
We exchange again and get:
\begin{align*}
  s_1 s_2 + (y^2 - r_2 m_2 y - k)^2 - (x - r_2)^2 s_1 - m_2^2 y^2 s_2
  &= 2 (m_2 x y - r_2 m_2 y - y^2 + r_2 m_2 y + k) \sqrt{s_1 s_2})\\
  &= 2 (m_2 x y - y^2 + k) \sqrt{s_1 s_2})
\end{align*}

\noindent
We raise again and get:
\begin{align*}
  (s_1 s_2 + (y^2 - r_2 m_2 y - k)^2 - (x - r_2)^2 s_1 - m_2^2 y^2 s_2)^2 = 4 (m_2 x y - y^2 + k)^2 s_1 s_2
\end{align*}

\noindent
We exchange and substitute and get:
\begin{align*}
  4 (m_2 x y - y^2 + k)^2 s_1 s_2
  &= ((d_1^2 - y^2) s_2 + (y^2 - r_2 m_2 y - k)^2 - (x - r_2)^2 (d_1^2 - y^2) - m_2^2 y^2 s_2)^2\\
  &= (\\
  & ~+ s_2 (d_1^2 - y^2 - m_2^2 y^2)\\
  & ~+ r_2^2 (y^2 - d_1^2 + m_2^2 y^2)\\
  & ~+ r_2 (2 m_2 k y - 2 m_2 y^3 + 2 (d_1^2 - y^2))\\
  & ~+ y^4 + k^2 - 2 k y^2 - d_1^2 x^2 + x^2 y^2\\
  & ~)^2\\
\end{align*}

We multiply by $(1 + m_2^2)^4$ and get:
\begin{align*}
  4 (m_2 x y - y^2 + k)^2 (1 + m_2^2)^4 s_1 s_2
  &= (\\
  & ~+ (1 + m_2^2)^2 s_2 (d_1^2 - y^2 - m_2^2 y^2)\\
  & ~+ (1 + m_2^2)^2 r_2^2 (y^2 - d_1^2 + m_2^2 y^2)\\
  & ~+ (1 + m_2^2)^2 r_2 (2 m_2 k y - 2 m_2 y^3 + 2 (d_1^2 - y^2))\\
  & ~+ (1 + m_2^2)^2 (y^4 + k^2 - 2 k y^2 - d_1^2 x^2 + x^2 y^2)\\
  & ~)^2\\
  &= (\\
  & ~+ (1 + m_2^2)^2 \frac{2 m_2 x y - y^2 + d_2^2 - m_2^2 x^2 + d_2^2 m_2^2}{(1 + m_2^2)^2} (d_1^2 - y^2 - m_2^2 y^2)\\
  & ~+ (1 + m_2^2)^2 \frac{(x + m_2 y)}{1 + m_2^2}^2 (y^2 - d_1^2 + m_2^2 y^2)\\
  & ~+ (1 + m_2^2)^2 \frac{(x + m_2 y)}{1 + m_2^2} (2 m_2 k y - 2 m_2 y^3 + 2 (d_1^2 - y^2))\\
  & ~+ (1 + m_2^2)^2 (y^4 + k^2 - 2 k y^2 - d_1^2 x^2 + x^2 y^2)\\
  & ~)^2\\
  &= (\\
  & ~+ (2 m_2 x y - y^2 + d_2^2 - m_2^2 x^2 + d_2^2 m_2^2) (d_1^2 - y^2 - m_2^2 y^2)\\
  & ~+ (x + m_2 y)^2 (y^2 - d_1^2 + m_2^2 y^2)\\
  & ~+ (1 + m_2^2) (x + m_2 y) (2 m_2 k y - 2 m_2 y^3 + 2 (d_1^2 - y^2))\\
  & ~+ (1 + m_2^2)^2 (y^4 + k^2 - 2 k y^2 - d_1^2 x^2 + x^2 y^2)\\
  & ~)^2\\
  &= (\\
  & ~+ 2 d_1^2 m_2 x y - d_1^2 y^2 + d_1^2 d_2^2 - d_1^2 m_2^2 x^2 + d_1^2 d_2^2 m_2^2\\
  & ~- 2 m_2 x y^3 + y^4 - d_2^2 y^2 + m_2^2 x^2 y^2 - d_2^2 m_2^2y^2\\
  & ~- 2 m_2^3 x y^3 + m_2^2 y^4 - d_2^2 m_2^2 y^2 + m_2^4 y^4 - d_2^2 m_2^4 y^2\\
  & ~+ y^2 x^2 - d_1^2 x^2 + m_2^2 x^2 y^2\\
  & ~+ m_2^2 y^4 - d_1^2 m_2^2 y^2 + m_2^4 y^4\\
  & ~+ 2 m_2 x y^3 - 2 d_1^2 m_2 x y - 2 m_2^3 x y^3\\
  & ~+ (x + m_2 y + m_2^2 x + m_2^3 y) (2 m_2 k y - 2 m_2 y^3 + 2 d_1^2 - 2 y^2)\\
  & ~+ (1 + m_2^4 + 2 m_2^2) (y^4 + k^2 - 2 k y^2 - d_1^2 x^2 + x^2 y^2)\\
  & ~)^2\\
\end{align*}

\noindent
We expand and get:
\begin{align*}
  4 (m_2 x y - y^2 + k)^2 (1 + m_2^2)^4 s_1 s_2
  &= (\\
  & ~+ 2 d_1^2 m_2 x y - d_1^2 y^2 + d_1^2 d_2^2 - d_1^2 m_2^2 x^2 + d_1^2 d_2^2 m_2^2\\
  & ~- 2 m_2 x y^3 + y^4 - d_2^2 y^2 + m_2^2 x^2 y^2 - d_2^2 m_2^2y^2\\
  & ~- 2 m_2^3 x y^3 + m_2^2 y^4 - d_2^2 m_2^2 y^2 + m_2^4 y^4 - d_2^2 m_2^4 y^2\\
  & ~+ y^2 x^2 - d_1^2 x^2 + m_2^2 x^2 y^2\\
  & ~+ m_2^2 y^4 - d_1^2 m_2^2 y^2 + m_2^4 y^4\\
  & ~+ 2 m_2 x y^3 - 2 d_1^2 m_2 x y - 2 m_2^3 x y^3\\
  & ~+ 2 m_2 k x y - 2 m_2 x y^3 + 2 d_1^2 x - 2 x y^2\\
  & ~+ 2 m_2^2 k y^2 - 2 m_2^2 y^4 + 2 d_1^2 m_2 y - 2 m_2 y^3\\
  & ~+ 2 m_2^3 k x y - 2 m_2^3 x y^3 + 2 d_1^2 m_2^2 x - 2 m_2^2 x y^2\\
  & ~+ 2 m_2^4 k y^2 - 2 m_2^4 y^4 + 2 d_1^2 m_2^3 y - 2 m_2^3 y^3\\
  & ~+ y^4 + k^2 - 2 k y^2 - d_1^2 x^2 + x^2 y^2\\
  & ~+ m_2^4 y^4 + k^2 m_2^4 - 2 m_2^4 k y^2 - d_1^2 m_2^4 x^2 + m_2^4 x^2 y^2\\
  & ~+ 2 m_2^2 y^4 + 2 k^2 m_2^2 - 4 m_2^2 k y^2 - 2 d_1^2 m_2^2 x^2 + 2 m_2^2 x^2 y^2\\
  & ~)^2
\end{align*}

\noindent
We regroup and get:
\begin{align*}
  4 (m_2 x y - y^2 + k)^2 (1 + m_2^2)^4 s_1 s_2
  &= 4 (m_2 x y - y^2 + k)^2 (1 + m_2^2)^4 (d_1^2 - y^2) \frac{2 m_2 x y - y^2 + d_2^2 - m_2^2 x^2 + d_2^2 m_2^2}{(1 + m_2^2)^2}\\
  &= 4 (m_2 x y - y^2 + k)^2 (1 + m_2^2)^2 (d_1^2 - y^2) (2 m_2 x y - y^2 + d_2^2 - m_2^2 x^2 + d_2^2 m_2^2)\\
  &= 4\\
  &  (m_2 x y - y^2 + k)^2 \\
  &  (1 + m_2^2)^2 \\
  &  (d_1^2 - y^2) \\
  &  (2 m_2 x y - y^2 + d_2^2 - m_2^2 x^2 + d_2^2 m_2^2)\\
  &= 4\\
  &  (m_2^2 x^2 y^2 + y^4 + k^2 - 2 m_2 x y^3 + 2 m_2 k x y - 2 k y^2) \\
  &  (1 + m_2^4 + 2 m_2^2) \\
  &  (d_1^2 - y^2) \\
  &  (2 m_2 x y - y^2 + d_2^2 - m_2^2 x^2 + d_2^2 m_2^2)\\
  &= 4\\
  & + (d_1^2 m_2^2 x^2 y^2 + d_1^2 y^4 + d_1^2 k^2 - 2 m_2 d_1^2 x y^3 + 2 m_2 d_1^2 k x y - 2 kd_1^2  y^2\\
  & + d_1^2 m_2^6 x^2 y^2 + d_1^2 m_2^4 y^4 + d_1^2 m_2^4 k^2 - 2 d_1^2 m_2 m_2^4 x y^3 + 2 d_1^2 m_2 m_2^4 k x y - 2 d_1^2 m_2^4 k y^2\\
  & + 2 d_1^2 m_2^24 x^2 y^2 + 2 d_1^2 m_2^2 y^4 + 2 d_1^2 m_2^2 k^2 - 4 d_1^2 m_2^3 x y^3 + 4 d_1^2 m_2^3 k x y - 4 d_1^2 m_2^2 k y^2\\
  & - m_2^2 x^2 y^4 - y^6 - k^2 y^2 + 2 m_2 x y^5 - 2 m_2 k x y^3 + 2 k y^4\\
  & - m_2^6 x^2 y^4 - m_2^4 y^6 - m_2^4 k^2 y^2 + 2 m_2 m_2^4 x y^5 - 2 m_2 m_2^4 k x y^3 +- 2 m_2^4 k y^4\\
  & - 2 m_2^24 x^2 y^3 - 2 m_2^2 y^6 - 2 m_2^2 k^2 +y^2  4 m_2^3 x y^5 - 4 m_2^3 k x y^3 + 4 m_2^2 k y^4)\\
  & (2 m_2 x y - y^2 + d_2^2 - m_2^2 x^2 + d_2^2 m_2^2)\label{eq:final}
 \end{align*}

% -----------------------------------------------------------------------------
\subsection{Simplifying}
\label{ssec:derivation-matlab}
% -----------------------------------------------------------------------------
We simplify last equation using Matlab. We obtain the bivariate
polynomial $P_2$, the zero set of which represents the points
satisfying the equation. We employ Matlab yet again to factorize the
polynomial $P_2$; see Section~\ref{ssec:derivation-p2} for the final
expressions. The Matlab script is available at
\url{http://acg.cs.tau.ac.il/projects/in-house-projects/localization-with-few-distance-measurements/solution.m}.

% -----------------------------------------------------------------------------
\subsection{Constraining the Slopes of Two Lines}
\label{ssec:derivation-constraining-slopes}
% -----------------------------------------------------------------------------

% -----------------------------------------------------------------------------
\subsection{The Result}
\label{ssec:derivation-p2}
% -----------------------------------------------------------------------------
The bivariate polynomial obtained by simplifying the system equation in the case where $L_1$ lies on the $x$-axis and and the intersection point of $L_1$ and $L_2$ coincides with the origin follows.

\begin{alignat*}{3}
  & P_2 && : && 4 \cdot k^2 \cdot y^4
    - 4 \cdot k^3 \cdot y^2
    + k^4 + d_1^4 \cdot d_2^4
    + 2 \cdot k^4 \cdot m_2^2
    + k^4 \cdot m_2^4
    + d_1^4 \cdot y^4
    + d_2^4 \cdot y^4 -\\
  & && && 4 \cdot d_1^2 \cdot k \cdot y^4
    - 4 \cdot d_2^2 \cdot k \cdot y^4
    - 2 \cdot d_1^2 \cdot d_2^2 \cdot k^2
    + 2 \cdot d_1^2 \cdot d_2^2 \cdot y^4
    - 2 \cdot d_1^2 \cdot d_2^4 \cdot y^2 -\\
  & && && 2 \cdot d_1^4 \cdot d_2^2 \cdot y^2
    + 2 \cdot d_1^2 \cdot k^2 \cdot y^2
    + 2 \cdot d_2^2 \cdot k^2 \cdot y^2
    + d_1^4 \cdot m_2^4 \cdot x^4
    + 2 \cdot d_2^4 \cdot m_2^2 \cdot y^4 +\\
  & && && d_2^4 \cdot m_2^4 \cdot y^4
    - 4 \cdot k^3 \cdot m_2^2 \cdot y^2
    + 4 \cdot k^2 \cdot m_2^2 \cdot y^4
    + 4 \cdot d_1^2 \cdot d_2^2 \cdot k \cdot y^2 - \\
  & && && 4 \cdot d_2^2 \cdot k \cdot m_2^2 \cdot y^4
    - 4 \cdot d_1^4 \cdot m_2^3 \cdot x^3 \cdot y
    - 8 \cdot k^2 \cdot m_2^3 \cdot x \cdot y^3
    - 2 \cdot d_1^2 \cdot d_2^2 \cdot k^2 \cdot m_2^2 +\\
  & && && 4 \cdot k^3 \cdot m_2 \cdot x \cdot y
    - 2 \cdot d_1^4 \cdot d_2^2 \cdot m_2^2 \cdot x^2
    - 2 \cdot d_1^2 \cdot d_2^2 \cdot m_2^2 \cdot y^4
    - 2 \cdot d_1^2 \cdot d_2^4 \cdot m_2^2 \cdot y^2+\\
  & && && 2 \cdot d_1^2 \cdot k^2 \cdot m_2^2 \cdot x^2
    - 2 \cdot d_1^2 \cdot k^2 \cdot m_2^4 \cdot x^2
    - 2 \cdot d_1^2 \cdot k^2 \cdot m_2^2 \cdot y^2
    - 2 \cdot d_2^2 \cdot k^2 \cdot m_2^4 \cdot y^2 +\\
  & && && 6 \cdot d_1^4 \cdot m_2^2 \cdot x^2 \cdot y^2
    + 4 \cdot k^2 \cdot m_2^2 \cdot x^2 \cdot y^2
    + 4 \cdot k^2 \cdot m_2^4 \cdot x^2 \cdot y^2
    - 4 \cdot d_1^4 \cdot m_2 \cdot x \cdot y^3 -\\
  & && && 8 \cdot k^2 \cdot m_2 \cdot x \cdot y^3
    + 4 \cdot k^3 \cdot m_2^3 \cdot x \cdot y
    + 4 \cdot d_1^2 \cdot d_2^2 \cdot m_2^3 \cdot x \cdot y^3
    - 12 \cdot d_1^2 \cdot k \cdot m_2^2 \cdot x^2 \cdot y^2 +\\
  & && && 4 \cdot d_1^4 \cdot d_2^2 \cdot m_2 \cdot x \cdot y
    - 4 \cdot d_1^2 \cdot k^2 \cdot m_2 \cdot x \cdot y
    + 12 \cdot d_1^2 \cdot k \cdot m_2 \cdot x \cdot y^3 +\\
  & && && 4 \cdot d_2^2 \cdot k \cdot m_2 \cdot x \cdot y^3
    + 2 \cdot d_1^2 \cdot d_2^2 \cdot m_2^2 \cdot x^2 \cdot y^2
    - 2 \cdot d_1^2 \cdot d_2^2 \cdot m_2^4 \cdot x^2 \cdot y^2 -\\
  & && && 4 \cdot d_1^2 \cdot d_2^2 \cdot m_2 \cdot x \cdot y^3
    + 4 \cdot d_1^2 \cdot k^2 \cdot m_2^3 \cdot x \cdot y
    + 4 \cdot d_1^2 \cdot k \cdot m_2^3 \cdot x^3 \cdot y +\\
  & && && 4 \cdot d_2^2 \cdot k \cdot m_2^3 \cdot x \cdot y^3
    + 8 \cdot d_1^2 \cdot d_2^2 \cdot k \cdot m_2^2 \cdot y^2
    - 8 \cdot d_1^2 \cdot d_2^2 \cdot k \cdot m_2^3 \cdot x \cdot y -\\
  & && && 4 \cdot d_1^2 \cdot d_2^2 \cdot k \cdot m_2 \cdot x \cdot y\\
  & && =\quad && (A_1\cdot x^2 + B_1\cdot y^2 + C_1\cdot x \cdot y + D_1)\cdot
    (A_2\cdot x^2 + B_2\cdot y^2 + C_2\cdot x \cdot y + D_2),\\
  \end{alignat*}
%
where\\
\begin{minipage}[c]{0.5\textwidth}
\begin{align*}
  A_1 &= d_1^2\cdot m_2^2\\
  B_1 &= d_1^2+d_2^2-2\cdot k+d_2^2\cdot m_2^2+2\cdot m_2\cdot e\\
  C_1 &= 2\cdot m_2\cdot (k - d_1^2 - m_2\cdot e)\\
  D_1 &= k^2 - d_1^2\cdot d_2^2 - k^2\cdot m_2^2 - 2\cdot k\cdot m_2\cdot e\\
\end{align*}
\end{minipage}
%
\begin{minipage}[c]{0.5\textwidth}
\begin{align*}
  A_2 &= d_1^2\cdot m_2^2\\
  B_2 &= d_1^2 - 2\cdot k + d_2^2 + d_2^2\cdot m_2^2 - 2\cdot m_2\cdot  e\\
  C_2 &= 2\cdot m_2\cdot (k - d_1^2 + m_2\cdot  e)\\
  D_2 &= k^2 - d_1^2\cdot d_2^2 - k^2\cdot m_2^2 + 2\cdot k\cdot m_2\cdot e\\
\end{align*}
\end{minipage}
and $e = \sqrt{d_1^2\cdot d_2^2 - k^2}$.
