\documentclass{article}
\usepackage[fleqn]{amsmath}
\usepackage{tikz}
\tikzset{%
  point/.style={circle,inner sep=1.25pt,minimum size=1.25pt,draw,fill=#1},
  point/.default=red
}
\definecolor{c0}{rgb}{0.2,0.4,0.67}
\definecolor{c1}{rgb}{0.67,0.4,0.12}
\definecolor{c2}{rgb}{0.53,0.6,0.13}
\definecolor{c3}{rgb}{0.53,0.53,0.4}
\begin{document}
\section{General Case}
\begin{align*}
  a_1 x_1 + b_1 y_1 + c_1 & = 0\\
  a_1 x_2 + b_1 y_2 + c_1 & = 0\\
  (x - x_1)^2 + (y - y_1)^2 & = d_1^2\\
  (x - x_2)^2 + (y - y_2)^2 & = d_2^2\\
  (x_2 - x_1)^2 + (y_2 - y_1)^2 & = d_1^2 + d_2^2 - 2 c d_1 d_2 = d_1^2 + d_2^2 - 2 k
\end{align*}
\section{Without Translation ($c_1 = c_2 = 0$)}
\begin{align*}
  y_1 & = m_1 x_1\\
  y_2 & = m_2 x_2\\
  (x - x_1)^2 + (y - m_1 x_1)^2 & = d_1^2\\
  (x - x_2)^2 + (y - m_2 x_2)^2 & = d_2^2\\
  (x_2 - x_1)^2 + (m_2 x_2 - m_1 x_1)^2 & = d_1^2 + d_2^2 - 2 k
\end{align*}
\begin{align*}
  x^2 + x_1^2 - 2 x x_1 + y^2 + m_1^2x_1^2 - 2 m_1 y x_1 &= d_1^2\\
  (1 + m_1^2) x_1^2 - 2 (x + m_1 y) x_1  + x^2 + y^2  &= d_1^2\\
  (1 + m_2^2) x_2^2 - 2 (x + m_2 y) x_2  + x^2 + y^2  &= d_2^2\\
  x_2^2 + x_1^2 - 2 x_1 x_2 + m_1^2 x_1^2 + m_2^2 x_2^2 - 2 m_1 m_2 x_1 x_2 &= d_1^2 + d_2^2 - 2 k\\
  (1 + m_1^2) x_1^2 + (1 + m_2^2) x_2^2 - 2 (1 + m_1 m_2) x_1 x_2 &= d_1^2 + d_2^2 - 2 k\\
\end{align*}
\begin{align*}
  x_1 &= \frac{x + m_1 y \pm \sqrt{(x + m_1 y)^2 - (1 + m_1^2)(x^2 + y^2 - d_1^2)}}{1 + m_1^2}\\
  x_2 &= \frac{x + m_2 y \pm \sqrt{(x + m_2 y)^2 - (1 + m_2^2)(x^2 + y^2 - d_2^2)}}{1 + m_2^2}\\
\end{align*}
\begin{align*}
  2 (1 + m_1 m_2) x_1 x_2 - 2 (x + m_1 y) x_1 - 2 (x + m_2 y) x_2 + 2 x^2 + 2 y^2 &= 2 k\\
  (1 + m_1 m_2) x_1 x_2 - (x + m_1 y) x_1 - (x + m_2 y) x_2 + x^2 + y^2 - k &= 0\\
\end{align*}
%% Symbolic
\section{Symbolic}
\begin{align*}
  x_1 &= r_1 \pm \sqrt{s_1}\\
  x_2 &= r_2 \pm \sqrt{s_2}\\
\end{align*}
\begin{align*}
  (1 + m_1 m_2) (r_1 \pm \sqrt{s_1}) (r_2 \pm \sqrt{s_2}) - (x + m_1 y) (r_1 \pm \sqrt{s_1}) - (x + m_2 y) (r_2 \pm \sqrt{s_2}) + x^2 + y^2 - k &= 0\\
\end{align*}
\begin{align*}
  (1 + m_1 m_2) (r_1 r_2 \pm r_1 \sqrt{s_2} \pm r_2 \sqrt{s_1} + \sqrt{s_1 s_2})\\
  - r_1 (x + m_1 y) \mp (x + m_1 y)\sqrt{s_1}\\
  - r_2 (x + m_2 y) \mp (x + m_2 y)\sqrt{s_2}\\
  + x^2 + y^2 - k &= 0\\
\end{align*}
\begin{align*}
  \pm r_1 (1 + m_1 m_2) \sqrt{s_2}
  \mp (x + m_2 y)\sqrt{s_2}\\
  \pm r_2 (1 + m_1 m_2) \sqrt{s_1}
  \mp (x + m_1 y)\sqrt{s_1}\\
  + (1 + m_1 m_2) \sqrt{s_1 s_2}
  - r_1 (x + m_1 y) \\
  - r_2 (x + m_2 y) \\
  + x^2 + y^2 - k &= 0\\
\end{align*}
\begin{align*}
  \pm (r_1 + r_1 m_1 m_2 - x - m_2 y) \sqrt{s_2} \pm (r_2 + r_2 m_1 m_2 - x - m_1 y) \sqrt{s_1} &=\\
  + (1 + m_1 m_2) \sqrt{s_1 s_2} - r_1 (x + m_1 y) - r_2 (x + m_2 y) + x^2 + y^2 - k\\
\end{align*}
\begin{align*}
  (r_1 + r_1 m_1 m_2 - x - m_2 y)^2 s_2 +  (r_2 + r_2 m_1 m_2 - x - m_1 y)^2 s_1\\
  + 2 ((r_1 + r_1 m_1 m_2 - x - m_2 y) (r_2 + r_2 m_1 m_2 - x - m_1 y) \sqrt{s_1} \sqrt{s_2}) &= \\
  + (1 + m_1 m_2)^2 s_1 s_2 + (x^2 + y^2 - r_1 (x + m_1 y) - r_2 (x + m_2 y) - k)^2\\
  + 2 (- r_1 (x + m_1 y) - r_2 (x + m_2 y) + x^2 + y^2 - k) (1 + m_1 m_2) \sqrt{s_1 s_2}\\
\end{align*}
\begin{align*}
  + 2 ((r_1 + r_1 m_1 m_2 - x - m_2 y) (r_2 + r_2 m_1 m_2 - x - m_1 y) \sqrt{s_1 s_2})\\
  + 2 (r_1 (x + m_1 y) + r_2 (x + m_2 y) - x^2 - y^2 + k) (1 + m_1 m_2) \sqrt{s_1 s_2} &= \\
  + (1 + m_1 m_2)^2 s_1 s_2 + (x^2 + y^2 - r_1 (x + m_1 y) - r_2 (x + m_2 y) - k)^2\\
  - (r_1 + r_1 m_1 m_2 - x - m_2 y)^2 s_2
  - (r_2 + r_2 m_1 m_2 - x - m_1 y)^2 s_1\\
\end{align*}
\begin{align*}
  + 2 ((r_1 + r_1 m_1 m_2 - x - m_2 y) (r_2 + r_2 m_1 m_2 - x - m_1 y) \sqrt{s_1 s_2})\\
  + 2 (r_1 (x + m_1 y) + r_2 (x + m_2 y) - x^2 - y^2 + k) (1 + m_1 m_2) \sqrt{s_1 s_2} &= \\
  + (1 + m_1 m_2)^2 s_1 s_2 + (x^2 + y^2 - r_1 (x + m_1 y) - r_2 (x + m_2 y) - k)^2\\
  - (r_1 + r_1 m_1 m_2 - x - m_2 y)^2 s_2
  - (r_2 + r_2 m_1 m_2 - x - m_1 y)^2 s_1\\
\end{align*}
%% x-Axis Aligned
\section{$x$-Axis Aligned}
\begin{align*}
  (r_1 \pm \sqrt{s_1}) (r_2 \pm \sqrt{s_2}) - x (r_1 \pm \sqrt{s_1}) - (x + m_2 y) (r_2 \pm \sqrt{s_2}) + x^2 + y^2 - k &= 0\\
\end{align*}
\begin{align*}
  r_1 r_2 \pm r_1 \sqrt{s_2} \pm r_2 \sqrt{s_1} + \sqrt{s_1 s_2}
  - x r_1 \mp x \sqrt{s_1} - r_2 (x + m_2 y) \mp (x + m_2 y) \sqrt{s_2}) + x^2 + y^2 - k &= 0\\
\end{align*}
\begin{align*}
  + \sqrt{s_1 s_2}
  + r_1 r_2 - x r_1 - r_2 (x + m_2 y)
  + x^2 + y^2 - k &=
  \mp r_2 \sqrt{s_1}
  \pm x \sqrt{s_1}
  \mp r_1 \sqrt{s_2}
  \pm (x + m_2 y) \sqrt{s_2})
\end{align*}
\begin{align*}
  + \sqrt{s_1 s_2}
  + r_1 r_2 - x r_1 - r_2 (x + m_2 y) + x^2 + y^2 - k &=
  \pm (x - r_2) \sqrt{s_1}
  \pm (x + m_2 y - r_1) \sqrt{s_2}
\end{align*}
\begin{align*}
  + s_1 s_2 + (r_1 r_2 - x r_1 - r_2 (x + m_2 y) + x^2 + y^2 - k)^2
  + 2 (r_1 r_2 - x r_1 - r_2 (x + m_2 y) + x^2 + y^2 - k) \sqrt{s_1 s_2} &=\\
  + (x - r_2)^2 s_1 + (x + m_2 y - r_1)^2 s_2 + 2 (x - r_2) (x + m_2 y - r_1) \sqrt{s_1 s_2}\\
\end{align*}
\begin{align*}
  + s_1 s_2 + (r_1 r_2 - x r_1 - r_2 (x + m_2 y) + x^2 + y^2 - k)^2 - (x - r_2)^2 s_1 - (x + m_2 y - r_1)^2 s_2 &=\\
  + 2 \sqrt{s_1 s_2} (r_2 x - r_1 x - y^2 + m_2 x y + k)\\
\end{align*}
\begin{align*}
  + (s_1 s_2 + (r_1 r_2 - r_1 x - r_2 x - r_2 m_2 y + x^2 + y^2 - k)^2 - (x - r_2)^2 s_1 - (x + m_2 y - r_1)^2 s_2)^2 &=\\
  + 4 (r_2 x - r_1 x - y^2 + m_2 x y + k)^2 s_1 s_2 \\
\end{align*}
%% Axis Aligned
\section{Axis Aligned}
\begin{align*}
  y_1 & = 0\\
  x_2 & = 0\\
  (x - x_1)^2 + y^2 &= d_1^2\\
  x^2 + (y - y_2)^2 &= d_2^2\\
  x_1^2 + y_2^2 &= d_1^2 + d_2^2 - 2 c d_1 d_2 = d_1^2 + d_2^2 - 2 k
\end{align*}
\begin{align*}
  x_1^2 - 2 x x_1 + x^2 + y^2 - d_1^2 &= 0\\
  y_2^2 - 2 y y_2 + x^2 + y^2 - d_2^2 &= 0\\
\end{align*}
\begin{align*}
  x_1 &= x + \sqrt{d_1^2 - y^2)}\\
  y_2 &= y + \sqrt{d_2^2 - x^2)}
\end{align*}
\begin{align*}
  x_1^2 + y_2^2 &= d_1^2 + d_2^2 - 2 k\\
  (x \pm \sqrt{d_1^2 - y^2)})^2 + (y \pm \sqrt{d_2^2 - x^2)})^2 &= d_1^2 + d_2^2 - 2 k\\
  x^2 + d_1^2 - y^2 + y^2 + d_2^2 - x^2 \pm 2 x \sqrt{d_1^2 - y^2)} \pm 2 y \sqrt{d_2^2 - x^2)} &= d_1^2 + d_2^2 - 2 k\\
  \pm x \sqrt{d_1^2 - y^2)} \pm y \sqrt{d_2^2 - x^2)} &= -k\\
  x^2 (d_1^2 - y^2) + y^2 (d_2^2 - x^2) \pm 2 x y \sqrt{d_1^2 - y^2)} \sqrt{d_2^2 - x^2)} &= k^2
\end{align*}
\begin{align*}
  \pm 2 x y \sqrt{(d_1^2 - y^2)(d_2^2 - x^2)} &= k^2 - x^2 (d_1^2 - y^2) - y^2 (d_2^2 - x^2)\\
  4 x^2 y^2 (d_1^2 - y^2)(d_2^2 - x^2) &= (k^2 - d_1^2x^2 + x^2y^2 - d_2^2y^2 + x^2y^2)^2\\
  4 x^2 y^2 (d_1^2d_2^2 - d_1^2x^2 - d_2^2y^2 + x^2y^2) &= (k^2 - d_1^2 x^2 - d_2^2 y^2 + 2 x^2 y^2)^2\\
  4 d_1^2d_2^2 x^2 y^2 - 4 d_1^2 x^4 y^2 - 4 d_2^2 x^2 y^4 + 4 x^4 y^4  &= k^4 + d_1^4 x^4 + d_2^4 y^4 2 + 4 x^4 y^4 \\
                                                                    &- 2 d_1^2 k^2 x^2 - 2 d_2^2 k^2 y^2 + 4 k^2 x^2 y^2 \\
                                                                    &+ 2 d_1^2 d_2^2 x^2 y^2 - 4 d_1^2 x^4 y^2 - 4 d_2^2 x^2 y^4 \\
  %
  d_1^4 x^4 + d_2^4 y^4 - 2 d_1^2 k^2 x^2 - 2 d_2^2 k^2 y^2 + 4 k^2 x^2 y^2 - 2 d_1^2d_2^2 x^2 y^2 + k^4 &= 0
\end{align*}
\begin{align*}
  (A_1 x^2 + B_1 y^2 + C_1 x y + D_1)(A_2 x^2 + B_2 y^2 + C_2 x y + D_2) &= 0\\
  A_1 A_2 X^4 + B_1 B_2 y^4 + (A_1 C_2 + A_2 C_1) x^3 y + (B_1 C_2 + B_2 C_1) x y^3 + \\
  (A_1 B_2 + A_2 B_1 + c_1 C_2) x^2 y^2 + (A_1 D_2 + A_2 D_1) x^2 + (B_1 D_2 + B_2 D_1) y^2 + \\
  (C_2 D_1 + C_1 D_2) x y + D_1 D_2 &= 0
\end{align*}
\begin{align*}
  A_1 A_2 &= d_1^4\\
  B_1 B_2 &= d_2^4\\
  A_1 C_2 + A_2 C_1 &= 0\\
  B_1 C_2 + B_2 C_1 &= 0\\
  A_1 B_2 + A_2 B_1 + C_1 C_2 &= 4 k^2 - 2 d_1^2 d_2^2\\
  A_1 D_2 + A_2 D_1 &= 2 -d_1^2 k^2\\
  B_1 D_2 + B_2 D_1 &= 2 -d_2^2 k^2\\
  C_2 D_1 + C_1 D_2 &= 0\\
  D_1 D_2 &= k^4
\end{align*}
\begin{align*}
  A_1 &= A_2 = d_1^2\\
  B_1 &= B_2 = d_2^2\\
  C_1 &= -C_2 = 2 \sqrt{d_1^2 d_2^2 - k^2}\\
  D_1 &= D_2 = -k^2\\
\end{align*}
%% Orthogonal
\section{Orthogonal ($m_1 m_2 = -1$)}
\begin{align*}
  2 x^2 + 2 y^2 - 2 (x + m_1 y) x_1 - 2 (x + m_2 y) x_2 &= 2 k\\
  (x + m_1 y) x_1 + (x + m_2 y) x_2 &= x^2 + y^2 - k\\
  (1 + m_1^2) x_1^2 - 2 (x + m_1 y) x_1  + x^2 + y^2 - d_1^2 &= 0\\
  (1 + m_2^2) x_2^2 - 2 (x + m_2 y) x_2  + x^2 + y^2 - d_2^2 &= 0\\
\end{align*}
\begin{align*}
  x_1 &= \frac{x + m_1 y + \sqrt{(x + m_1 y)^2 - (1 + m_1^2)(x^2 + y^2 - d_1^2)}}{1 + m_1^2}\\
      &= \frac{x + m_1 y + \sqrt{x^2 + y^2 m_1^2 + 2 m_1 x y - x^2 - y^2 + d_1^2 - m_1^2 x^2 - m_1^2 y^2 + m_1^2 d_1^2}}{1 + m_1^2}\\
      &= \frac{x + m_1 y + \sqrt{2 m_1 x y - y^2 + d_1^2 - m_1^2 x^2 + m_1^2 d_1^2}}{1 + m_1^2}\\
  x_2 &= \frac{x + m_2 y + \sqrt{2 m_2 x y - y^2 + d_2^2 - m_2^2 x^2 + m_2^2 d_2^2}}{1 + m_2^2}\\
\end{align*}
\begin{align*}
  (x + m_1 y) \frac{x + m_1 y + \sqrt{2 m_1 x y - y^2 + d_1^2 - m_1^2 x^2 + m_1^2 d_1^2}}{1 + m_1^2} &+ \\
  (x + m_2 y) \frac{x + m_2 y + \sqrt{2 m_2 x y - y^2 + d_2^2 - m_2^2 x^2 + m_2^2 d_2^2}}{1 + m_2^2} &= x^2 + y^2 - k\\
\end{align*}
\begin{align*}
  (1 + m_2^2)(x + m_1 y)(x + m_1 y + \sqrt{2 m_1 x y - y^2 + d_1^2 - m_1^2 x^2 + m_1^2 d_1^2}) &+ \\
  (1 + m_1^2)(x + m_2 y)(x + m_2 y + \sqrt{2 m_2 x y - y^2 + d_2^2 - m_2^2 x^2 + m_2^2 d_2^2}) &= \\
  (1 + m_1^2)(1 + m_2^2)(x^2 + y^2 - k)\\
  %
  (1 + m_2^2)(x + m_1 y)^2 + (1 + m_2^2)(x + m_1 y)\sqrt{2 m_1 x y - y^2 + d_1^2 - m_1^2 x^2 + m_1^2 d_1^2} &+ \\
  (1 + m_1^2)(x + m_2 y)^2 + (1 + m_1^2)(x + m_2 y)\sqrt{2 m_2 x y - y^2 + d_2^2 - m_2^2 x^2 + m_2^2 d_2^2} &= \\
  (1 + m_1^2)(1 + m_2^2)(x^2 + y^2 - k)\\
\end{align*}
\begin{align*}
  (1 + m_2^2)(x + m_1 y)\sqrt{2 m_1 x y - y^2 + d_1^2 - m_1^2 x^2 + m_1^2 d_1^2} &+ \\
  (1 + m_1^2)(x + m_2 y)\sqrt{2 m_2 x y - y^2 + d_2^2 - m_2^2 x^2 + m_2^2 d_2^2} &= \\
  (2 + m_2^2 + m_1^2)(x^2 + y^2 - k) - (1 + m_2^2)(x + m_1 y)^2 - (1 + m_1^2)(x + m_2 y)^2 \\
  &= \\
  2 x^2 + 2 y^2 - 2 k + m_1^2 x^2 + m_1^2 y^2 - m_1^2 k + m_2^2 x^2 + m_2^2 y^2 - m_2^2 k\\
  - (1 + m_2^2)(x^2 + m_1^2 y^2 + 2 m_1 x y) - (1 + m_1^2)(x^2 + m_2^2 y^2 + 2 m_2 x y)\\
  &= \\
  2 x^2 + 2 y^2 - 2 k + m_1^2 x^2 + m_1^2 y^2 - m_1^2 k + m_2^2 x^2 + m_2^2 y^2 - m_2^2 k\\
  - x^2 - m_1^2 y^2 - 2 m_1 x y - m_2^2 x^2 - m_1^2 m_2^2 y^2 - 2 m_1 m_2^2 x y\\
  - x^2 - m_2^2 y^2 - 2 m_2 x y - m_1^2 x^2 - m_1^2 m_2^2 y^2 - 2 m_1^2 m_2 x y\\
  &= - 2 k - m_1^2 k - m_2^2 k\\
\end{align*}
\begin{align*}
  (x + m_1 y + m_2^2 x - m_2 y) \sqrt{2 m_1 x y - y^2 + d_1^2 - m_1^2 x^2 + m_1^2 d_1^2} &+ \\
  (x + m_2 y + m_1^2 x - m_1 y) \sqrt{2 m_2 x y - y^2 + d_2^2 - m_2^2 x^2 + m_2^2 d_2^2} &= - 2 k - m_1^2 k - m_2^2 k\\
\end{align*}
%% Rotating Axis Aligned
\subsection{Rotating Axis Aligned}
\begin{align*}
  x' &= x \cos(\alpha) + y \sin(\alpha) = x \frac{1}{\sqrt{1+m_1^2}} + y \frac{m_1}{\sqrt{1+m_1^2}}\\
  y' &= x \sin(\alpha) - y \cos(\alpha) = x \frac{m_1}{\sqrt{1+m_1^2}} - y \frac{1}{\sqrt{1+m_1^2}}\\
\end{align*}
\begin{align*}
  A_1 x'^2 + B_1 y'^2 + C_1 x' y' + D_1 &= 0\\
  d_1^2 x'^2 + d_2^2 y'^2 + 2 \sqrt{d_1^2 d_2^2 - k^2} x' y' - k^2 &= 0\\
\end{align*}
\begin{align*}
  d_1^2 (x \frac{1}{\sqrt{1 + m_1^2}} + y \frac{m_1}{\sqrt{1 + m_1^2}})^2 +
  d_2^2 (x \frac{m_1}{\sqrt{1 + m_1^2}} - y \frac{1}{\sqrt{1 + m_1^2}})^2 &+\\
  2 \sqrt{d_1^2 d_2^2 - k^2} (x \frac{1}{\sqrt{1 + m_1^2}} + y \frac{m_1}{\sqrt{1 + m_1^2}}) (x \frac{m_1}{\sqrt{1 + m_1^2}} - y \frac{1}{\sqrt{1 + m_1^2}}) - k^2 &= 0\\
\end{align*}
\begin{align*}
  d_1^2 (\frac{x + m_1 y}{\sqrt{1+m_1^2}})^2 + d_2^2 (\frac{m_1 x - y}{\sqrt{1 + m_1^2}})^2 +
  2 \sqrt{d_1^2 d_2^2 - k^2} (\frac{x + m_1 y}{\sqrt{1 + m_1^2}}) (\frac{m_1 x - y}{\sqrt{1 + m_1^2}}) - k^2 &= 0\\
\end{align*}
\begin{align*}
  d_1^2 \frac{(x + m_1 y)^2}{1 + m_1^2} + d_2^2 \frac{(m_1 x - y)^2}{1 + m_1^2} +
  2 \sqrt{d_1^2 d_2^2 - k^2} \frac{(x + m_1 y)(m_1 x - y)}{1 + m_1^2} - k^2 &= 0\\
\end{align*}
\begin{align*}
  d_1^2 (x + m_1 y)^2 + d_2^2 (m_1 x - y)^2 +
  2 \sqrt{d_1^2 d_2^2 - k^2} (x + m_1 y)(m_1 x - y) - k^2 (1 + m_1^2) &= 0\\
\end{align*}
\begin{align*}
  d_1^2 (x^2 + m_1^2 y^2 + 2 m_1 x y) + d_2^2 (m_1^2 x^2 + y^2 - 2 m_1 x y) &+\\
  2 \sqrt{d_1^2 d_2^2 - k^2} (m_1 x^2 - x y + m_1^2 x y - m_1 y^2) - k^2 (1 + m_1^2) &= 0\\
\end{align*}
\begin{align*}
    d_1^2 (m_2 x^2 - m_1 y^2 - 2 x y) + d_2^2 (- m_1 x^2 + m_2 y^2 + 2 x y) &+\\
  2 \sqrt{d_1^2 d_2^2 - k^2} (- x^2 - m_2 x y - m_1 x y + y^2) - k^2 (m_2 - m_1) &= 0\\
\end{align*}
\begin{align*}
  (d_1^2 m_2 - d_2^2 m_1 - 2 \sqrt{d_1^2 d_2^2 - k^2}) x^2 +
  (d_2^2 m_2 - d_1^2 m_1 + 2 \sqrt{d_1^2 d_2^2 - k^2}) y^2 +\\
  2 (d_2^2 - d_1^2 - (m_1 + m_2) \sqrt{d_1^2 d_2^2 - k^2}) x y &+ k^2 (m_1 - m_2) &= 0\\
\end{align*}
\end{document}
